---
lastSync: Mon Mar 31 2025 11:34:41 GMT-0400 (Eastern Daylight Time)
---
## Lesson
- $$F_{g}=\frac{Gm_{1}m_{2}}{r^2}$$
- $$G=6.67 \times 19^{-11} \frac{Nm^2}{kg^2}=\text{universal gravitational constant}$$
- $$F_{g} \propto M \implies \frac{Fg_{1}}{M_{1}}=\frac{Fg^2}{M^2}$$
- $$F_{g} \propto \frac{1}{r^2} \implies Fg_{1}r^2_{1} = Fg_{2}r^2_{2}$$
## Examples
- 1. A 100kg astronaut get transported from 7 earth radius (re=6.38x10^6) to a new radius 10m greater. determine the change in gravitational force. (me=5.98x10^24)
	- Variables
		- m1=100kg
		- m2=5.98x10^24
		- r=7(6.38x10^6)
	- Equations
		- $$\Delta fg=fg_{2}-fg_{1}$$
		- $$\Delta fg=\frac{Gm_{1}m_{2}}{(7re+10)^2}-\frac{Gm_{1}m_{2}}{(7re)^2}$$
		- $$F_{g}=\frac{Gm_{1}m_{2}}{r^2}=kr^{-2}$$
		- $$\frac{dF}{dr}=-2kr^{-3}$$
		- $$dF=-2kr^{-3}dr$$
		- 
