---
lastSync: Thu Sep 18 2025 10:33:16 GMT-0400 (Eastern Daylight Time)
---
$$\begin{align}
KE & =\frac{1}{2}m_{1}v_{1}^2+\frac{1}{2}m_{2}v_{2}^2=\frac{1}{2}m_{1}v_{1_{f}}^2+\frac{1}{2}m_{2}v_{2_{f}}^2 \\
m_{1}(v_{1_{i}}-v_{1_{f}}) & =m_{2}(v_{2_{i}}-v_{2_f}) \\
m_{1}(v_{1_{i}}^2-v_{1_{f}}^2) & =m_{2}(v_{2_{i}}^2-v_{2_f}^2) \\
\frac{m_{1}(v_{1_{i}}^2-v_{1_{f}}^2)}{m_{1}(v_{1_{i}}-v_{1_{f}})} & =\frac{m_{2}(v_{2_{i}}^2-v_{2_f}^2)}{m_{2}(v_{2_{i}}-v_{2_f})} \\
m_{1}(v_{1_{i}}+v_{1_{f}}) & =m_{2}(v_{2_{i}}+v_{2_f}) \\
\end{align}$$
