---
lastSync: Fri Sep 26 2025 12:19:15 GMT-0400 (Eastern Daylight Time)
---
# Definitions
![[Pasted image 20250926113553.png]]
$$\begin{align}
 & \tanh x= \frac{\sinh x}{\cosh x}
\end{align}$$
## Example
![[Pasted image 20250926113807.png]]
$$\begin{align}
 & \cosh(\ln(t)) = \frac{e^{\ln t}+e^{-\ln t}}{2} \\
 & \cosh(\ln(t)) = \frac{t+\frac{1}{t}}{2} \\
 & \cosh(\ln(t)) = \frac{t^2+1}{2t}
\end{align}$$
![[Pasted image 20250926114205.png]]
$$\begin{align}
 & \lim_{ x \to \infty } \frac{\frac{e^x-e^{-x}}{2}}{\frac{e^x+e^{-x}}{2}}  \\
\iff & \lim_{x\to\infty}\frac{(e^{x}-e^{-x})}{(e^{x}+e^{-x})} \\
\iff & \lim_{ x \to \infty } \frac{\cancel{ e^x }(1-e^{-2x})}{\cancel{ e^x }(1+e^{-2x})} \\
\iff & \frac{1-0}{1+0} \\
\iff & \boxed{ 1 }
\end{align}$$
## Application: Hanging wire

![[Pasted image 20250926114847.png]]
# Identities
![[Pasted image 20250926114915.png]]
$$\begin{align}
 \sinh(-x) & =\frac{e^{-x}-e{-(-x)}}{2} \\
 & =\frac{e^{-x}-e^x}{2} \\
 & =-\left( \frac{e^x-e^{-x}}{2} \right) \\
 & =\boxed{ -\sinh x }
\end{align}$$
$$\begin{align}
\cosh^2x-\sinh^x &  =\frac{e^x+e^{-x}}{2}^2-\frac{e^x-e^{-x}}{2}^2 \\

 & =\frac{e^{2x}+2+e^{-2x}}{4}-\frac{e^{2x}-2+e^{-2x}}{4} \\
 & =\frac{4}{4} \\
 & =\boxed{ 1 }
\end{align}$$
# Why "Hyperbolic"?
$$\begin{align}
 & \text{Recall} \cosh^2t-\sinh^2t=1
\end{align}$$
![[Pasted image 20250926115532.png]]
# Derivatives
![[Pasted image 20250926115638.png]]
$$\begin{align}
\frac{d}{dx}\left( \frac{e^x+e^{-x}}{2} \right) & =\frac{e^x-e^{-x}}{2} \\
 & =\sinh x
\end{align}$$
# Inverse Hyperbolic Function
![[Pasted image 20250926120236.png]]
$$\begin{align}
y=\sinh x \iff \sinh^{-1}y=x
\end{align}$$
![[Pasted image 20250926120315.png]]
$$\begin{align}
 & \text{restrict domain to }x\geq 0 \implies \cosh^{-1}x=y \\
 & y=\cosh x \underbrace{ \iff }_{ \text{if }x \geq 0 } \cosh^{-1}y=x \\
 & \text{Suppose } a>0,Q:\cosh^{-1}(\cosh(-a))=a  & (=|-a|)
\end{align}$$
![[Pasted image 20250926120829.png]]
$$\begin{align}
y=\tanh x  & \iff \tanh^{-1}y=x \\
 & (-1 < y < 1 \text{ automatically})
\end{align}$$
![[Pasted image 20250926121036.png]]
$$\begin{align}
 & \sinh^{-1}x=? \\
 & y=\sinh x \\
\iff & y=\frac{e^x-e^{-x}}{2} \\
\iff & e^x-2y-e^{-x} \\
\iff  & 0=e^{2x}-2ye^x-1 \\ \\
 & \text{Write } t=e^x \\

\iff & 0=t^2-2yt-1 \\
 \\
 & \text{By quadratic formula} \\
 & t=\frac{2y \pm \sqrt{ 4y^2+4 }}{2} \\
 & t=y\pm \sqrt{ y^2+1 } \\
 \\
 & \text{recall: }t=e^x >0 \\
 & \text{note } y=\sqrt{ y^2-1 } <0  \\
 & \text{so only solution with "+" is valid in x} \\ \\

 & e^x=y+\sqrt{ y^2+1 } \\
\implies & x=\ln(y+\sqrt{ y^2+1 })
\end{align}$$