---
lastSync: Fri Sep 19 2025 12:14:44 GMT-0400 (Eastern Daylight Time)
---
# The chain rule
$$\begin{align}
 & \frac{d}{dx}(x^2+1) \to \text{easy, seen how to do this} \\
 &  \frac{d}{dx} \sqrt{ x }=\frac{1}{2\sqrt{ x }} \\

 & \frac{d}{dx} \sqrt{ x^2+1 }=\frac{1}{2\sqrt{ x^2+1 }}\times 2x
\end{align}$$
## The chain rule
Give g differentiable at x and f differentiable at g(x) then f(g(x)) is differentiable at x and $$\begin{align}
 & \boxed{ (f \circ g)'(x)=f'(g(x))g'(x) } \\ \\

 & \text{Memorization Trick} \\
 & \text{if }y=f(u) \text{ and } u=g(x) \\
 & \text{then } \boxed{ \frac{dy}{dx}=\frac{dy}{du} \times \frac{du}{dx} } \to \text{look up "back propagation"}
\end{align}$$ 