---
lastSync: Fri Sep 26 2025 11:35:13 GMT-0400 (Eastern Daylight Time)
---
# Derivative of the logarithm
$$\begin{align} 
 & y=\log_{b}x  & \frac{d}{dx}y=? \\
\iff & b^y=x \\
\implies & b^y \ln b \left( \frac{dy}{dx} \right) = 1 \\
\iff & \frac{dy}{dx}=\frac{1}{b^y\ln b} & b^x=x \\
\iff & \boxed{ \frac{d}{dx}(\log_{b}x)=\frac{1}{x\ln(b)}} \\
\implies &  \boxed{ \frac{d}{dx}\ln x =\frac{1}{x} } \\ \\

 & \text{More generally} \\
 & \boxed{ \frac{d}{dx} \ln(f(x))=\frac{f'(x)}{f(x)} }
\end{align}$$
# Examples
![[Pasted image 20250925115234.png]]
$$\begin{align}
\frac{d}{dx}\ln(\sin x) = \frac{\cos x}{\sin x}=\cot x
\end{align}$$
![[Pasted image 20250925115421.png]]
$$\begin{align}
 & \frac{d}{dx} \ln \left( \frac{x+1}{\sqrt{ x^2-2 }} \right) =\frac{d}{dx}(\ln(x+1)-\ln((x^2-2)^{1/2})) \\
& \frac{d}{dx} \ln \left( \frac{x+1}{\sqrt{ x^2-2 }} \right) =\frac{1}{x+1}-\frac{1}{2}\left( \frac{2x}{x^2-2} \right)

\end{align}$$
![[Pasted image 20250925115908.png]]
$$\begin{align}
 & \frac{d}{dx}(\ln|x|)=\begin{cases}
\ln(x) & x>0 \\
\ln(-x) & x<0
\end{cases} \\
 & \frac{d}{dx}(\ln(|x|)=\begin{cases}
\frac{1}{x} & x>0 \\
\frac{1}{(-x)}(-1) & x<0 \\

\end{cases} \\
 & \boxed{ \frac{d}{dx}\ln|x|=\frac{1}{x} }
\end{align}$$
![[Pasted image 20250925120154.png]]
$$\begin{align}
 & \frac{d}{dx}(x^\sqrt{ x })=\frac{d}{dx}e^{\ln x\times \sqrt{ x }} \\
 & \frac{d}{dx}(x^\sqrt{ x })=e^{\ln x\sqrt{ x }}\left( \frac{1}{x}\sqrt{ x }+\ln x \frac{1}{2\sqrt{x }} \right)
\end{align}$$
# Logarithmic Differentiation
![[Pasted image 20250925120507.png]]
$$\begin{align}
 & \text{Have }\ln(y)=\ln\left( x^{3/4} \frac{\sqrt{ x^2+1 }}{(x^2+2)^5} \right) \\
\implies & \frac{1}{y}y'=\frac{d}{dx}\underbrace{ \ln\left( x^{3/4} \frac{\sqrt{ x^2+1 }}{(x^2+2)^5} \right) }_{ x } \\
 & x=\frac{d}{dx}\left( \frac{3}{4}\ln x+\frac{1}{2}\ln(x^2+1)-5\ln(3x+2) \right) \\
 & x = \frac{3}{4} \frac{1}{x} +\frac{1}{2} \frac{2x}{x^2+1} -5 \frac{3}{3x+2} \\
 & y' = y\left( \frac{3}{4} \frac{1}{x} +\frac{1}{2} \frac{2x}{x^2+1} -5 \frac{3}{3x+2} \right) \\
 & y'=x^{3/4}\left( \frac{\sqrt{ x^2+1 }}{(3x+2)^5} \right)\left( \frac{3}{4x} +\frac{x}{x^2+1}-\frac{15}{3x+2} \right)
\end{align}$$
# A general formula
$$\begin{align}
 & y=f^{-1}(x)  & \to \frac{dy}{dx}=? \\
\implies & f(y)=x \\
\implies  & \frac{d}{dx}(f(y))=1 \\
\implies & f'(y)\times=1 \\
\implies & f'(f^{-1}(x))(f^{-1}(x))'=1 \\
\implies & \boxed{ f^{-1}(x)'=\frac{1}{f'(f^{-1}(x))} }
\end{align}$$
# Derivatives of inverse trig functions
![[Pasted image 20250925121406.png]]
$$\begin{align}
 & \frac{d}{dx}(\sin^{-1}x)=\frac{1}{\sin'(\sin^{-1}(x))} \\
 & \frac{d}{dx}(\sin^{-1}x) = \frac{1}{\cos(\underbrace{ \sin^{-1}(x) }_{ \theta })} \\ \\
 & \frac{x}{1}=\sin \theta \\
 & \to \cos \theta=\sqrt{ 1-x^2} \\
 & =\cos(\sin^{-1}x)=\sqrt{ 1-x^2 } \\
 \\
\frac{d}{dx}\sin^{-1}x=\frac{1}{\sqrt{ 1-x^2 }}
\end{align}$$
![[Pasted image 20250925121622.png]]
### Example
$$\begin{align}
 & \frac{d}{dx} \arctan x = \frac{1}{\sec^2(\underbrace{ \arctan x }_{ \theta })}  \\
 & 1+\tan ^2x=\sec ^2 \\
 & \frac{1}{(1+\tan ^2(\arctan x))} \\
 & \frac{1}{1+x^2}
\end{align}$$