---
lastSync: Mon Sep 29 2025 15:16:18 GMT-0400 (Eastern Daylight Time)
---
## Question 1
$$\begin{align}
 & \text{Find the value of y' when x=0 if} \\
 & xy^8+e^{y/6}=e \\
 & \text{y(x) is a function defined by y(x)=the y value that makes} \\
 & xy(x)^8+e^{y(x)/6}=e \text{ for the given x} \\
 \\
 & xy^8+e^{y/6}=e  & (1) \\ \\

 & \text{Differentiate both sides:} \\
 & \frac{d}{dx}\underbrace{ xy^8 }_{ \text{product rule} }+e^{y/6}=\frac{d}{dx}e \\
 & 1 \times y^8 + x \times \underbrace{ 8y^7 \times \frac{dy}{dx} }_{ \text{chain rule} }+e^{y/6} \times \frac{1}{6} \times \frac{dy}{dx} & e^{y(x)/6} \implies \frac{d}{dx} \frac{y}{6}e^{y(x)/6} \\
 & y^8+8xy^7 \times y' +\frac{1}{6} e^{y/6} y' = 0  & (2)\\
 \\
 & \text{If x=0, eqn (1) } \to e^{y/6}=e \implies y=6 \\
 & \text{eqn (2)} \to 6^8+\frac{e}{6}y'=0 \\
 & 
\end{align}$$
## Question 2
$$\begin{align}
 & \text{If } f(x+x^3[f(x)]=6x+4 \text{ and }f(1)=2, \text{find }f'(1) \\ \\

 & \frac{d}{dx}f(x+x^3[f(x)]=\frac{d}{dx}6x+4 \\
 & f'(x)+3x^2[f(x)]^3+x^3\times 3[f(x)]^2 \times f'(x)=6 \\ \\

 & \text{Sub } x=1 \\
 & f'(1)+3 \times 1^2 \times 2^3 +1^3 \times 3 \times 2^2 \times f'(1)=6 \\
 & f'(1)+24+12f'(1) =6 \\
 & 13f'(1)=-18 \\
 & \boxed{ f'(1)=-\frac{18}{13} }
\end{align}$$
## Question 3
$$\begin{align}
 & \text{Let} f(x)=\ln[1+g(x)] \text{ where } g(5)=e^7-1\text{ and } g'(5)=6e^7 \\
 & \text{Find eqn of tangent line to f at }x=5 \\ \\
 & \text{Recall}: \frac{d}{dx}\ln(x)=\frac{1}{x} \\
 & f'(x)=\frac{g'(x)}{1+g(x)} \\ \\

 & \text{Plug }x=5 \text{ into }f(x) \text{ to find a point on the line:} \\
 & f(5)=\ln(1+g(5))=\ln(\cancel{ 1 }+e^7\cancel{ -1 })=\ln e^7=7 \\
 \\
 & \text{Plug } x=5 \text{ into } f'(x) \text{ to find the slope of the line:} \\
 & f'(5)=\frac{g'(5)}{1+g(5)}=\frac{6e^7}{\cancel{ 1 }+e^7-\cancel{ 1 }}=\frac{6\cancel{ e^7 }}{\cancel{ e^7 }}=6 \\
 \\
 & \therefore \text{ eqn of tangent line at x=5 is } y=6x-23
\end{align}$$
## Question 4
$$\begin{align}
 & \text{Let }f(x)=(\tan^{-1}(\sqrt{ x }))^2\text{. Find f'(1)} \\
 & \text{Recall: } \frac{d}{dx}\tan^{-1}x=\frac{1}{1+x^2} \\
 & f'(x)=2\tan^{-1}(\sqrt{ x }) \times \frac{d}{dx} \tan^{-1}(\sqrt{ x })  \\
 & =2\tan^{-1}(\sqrt{ x }) \times \frac{1}{1+\sqrt{ x }^2} \times \frac{d}{dx} \sqrt{ x } \\
 & =\frac{2\tan^{-1}\sqrt{ x }}{1+x}\times \frac{1}{x}\sqrt{ x } \\
 & =\frac{\tan^{-1}\sqrt{ x }}{\sqrt{ x }(1+x)} \\
 & =\frac{\tan^{-1}\sqrt{ 1 }}{\sqrt{ 1 }(1+1)} \\
 & =\frac{\tan^{-1}1}{2} \\
 & = \frac{\pi}{8}
\end{align}$$
## Question 5
$$\begin{align}
 & \text{Let } f(x)=\sqrt{ x }^x\text{. Find }f'(4)4 \\
 \\
 & \mathbb{Use Logorithmic Differentiation} \\
 & \ln f(x)=\ln(\sqrt{ x }^x) & \frac{d}{dx}\ln f(x) =\frac{f'(x)}{f(x)}\\

 & =x\ln (x^{1/2}) \\
 & =\frac{x}{2}\ln x \\
 & = \frac{d}{dx} \frac{x}{2}\ln x \\
 & = \frac{1}{2}\ln x+\frac{\cancel{ x }}{2} \frac{1}{\cancel{ x }} \\
 & =\frac{\ln x+1}{2} \\
 & =\frac{f'(x)}{f(x)}=\frac{\ln x+1}{2} \\
 & f'(x)=\frac{\sqrt{ x }^x(\ln x+1)}{2} \\
 & f'(4)=\sqrt{ 4 }^4(\ln 4+1) \\
 & =8\ln 4+8
\end{align}$$
## Question 6
$$\begin{align}
 & \text{Suppose that f is 1-1, differentiable fn and }f^{-1} \text{ is also differentiable. Show that} \\
 & (f^{-1})'(x)=\frac{1}{f'(f^{-1}(x))} \\
 & \text{Provided that the denominator is not 0} \\
 \\
 & \text{Since f is 1-1, }f^{-1} \text{ is well defined. Now consider the curve }y=f(x) \iff f(y)=x\\
 & f'(y)\times y'=1 \\
 & f'(f^{-1}(x))\times(f^{-1}(x))=1 \\
 & (f^{-1}(x))'=\frac{1}{f'(f^{-1}(x))}
\end{align}$$