---
lastSync: Thu May 22 2025 11:00:28 GMT-0400 (Eastern Daylight Time)
---
## Lesson
![[Drawing 2025-05-22 10.35.42.excalidraw]]
- $$\begin{align}
\sum F & =ma \\
f(t)-k x(t)-b \dot{x}(t) & =m\ddot{x}(t) \\
\ddot{x}(t)-\frac{b}{m} \dot{x}(t)+\frac{k}{m}x(t) &= f(t) \\ \\

m=1, b=3, k=2 \\
 \\
\ddot{x}(t)+3 \dot{x}(t) + 2x(t)  & = f(t) \\
\ddot{x}(t)+3 \dot{x}(t) + 2x(t)  & = f(t) \implies \text{Leplace Transform} \implies s^2x(s)+3s x(s)+2x(s)=F(s) \\
 \\
X(s)[s^2+3s+2] & =F(s) \implies x(s)=\frac{F(s)}{s^2+3s+2} \implies \text{Inverse Lecplace Transform} \\
 \\
\text{Supposed } f(t) & =\text{unit step} \\
 \\
f(t) \implies LT \implies F(s) & =\frac{1}{s} \\
x(s) & =\frac{1}{(s^2+3s+2)} \implies ILT \implies x(t)=\frac{1}{2}e^{-2t}-e^{-t}+\frac{1}{2} \\
 \\ 
\end{align}$$
- Laplace Transform
- $$\begin{align}
x(s) & =y \{x(t)\}=\int_{0}^{\infty }\underbrace{ x(t)e^{-st}dt }_{ s\in\mathbb{C} } \\
\end{align}$$
- $$\begin{array}{rr}
f(t) & f(s) \\
f(t)=\text{unit step} & f(s)=\frac{1}{s} \\
f(t)=e^{at} & f(s)=\frac{1}{(s-a)} \\
f(t)=t^n & f(s)=\frac{n!}{s^{n+1}} \\
\end{array}$$
- $$x(\omega)=f\{x(t)\}=\int_{-\infty}^{\infty} x(t)e^{-j_{2}\pi \omega t} \, dx $$