## Defintion
Context: (very) long sums with a repeating pattern occur often and naturally in mathematics (see e.g. next lecture).

The summation symbol is an efficient notation that provides a principled way of working with such sums.

Defintion: given integers $\underbrace{ m\leq n }_{ i }$ and real numbers $\underbrace{ a_{m}\dots,a_{n} }_{ m,m+1\dots n-1,n }$ we write
$$\begin{align}
\sum^n_{i=m}\underbrace{ a_{i} }_{ \text{general term} }=a_{m}+a_{m+1}+\dots+a_{n-1}+a_{n}
\end{align}$$
## Examples: expand the following sums, where k is some natural numbers
$$\begin{align}
\sum^4_{i=1}i^2=\underbrace{ 1^2 }_{ 1 }+\underbrace{ 2^2 }_{ 2 }+\underbrace{ 3^2 }_{ 3 }+\underbrace{ 4^2 }_{ 4 } \\
 & =1+4+9+16 \\
 & \boxed{ =30 }
\end{align}$$
$$\begin{align}
\sum^{k+2}_{j=k}j \cdot k & =k\cdot \underbrace{ k }_{ k }+(\underbrace{ k+1)k }_{ k+1 }+\underbrace{ (k+2)k }_{ k+2 } \\
 & =3k^2+3k
\end{align}$$
## Examples: write in sigma natation
$$\begin{align}
4+9+16+25 & =\sum^5_{i=2}i^2 \\
 & = \sum ^3_{i=0}(2+n)^2 \\
 & =\sum^4_{k=1}(1+k)^2
\end{align}$$
$$\begin{align}
\frac{2}{3}+\frac{8}{5}+\frac{26}{7}+\frac{80}{9}= \sum _{n=1}^4= \frac{3^i-1}{2i+1} 
\end{align}$$
## Observation: changing summation indices
$$\begin{align}
\sum^n_{i=m}a_{i} & =a_{m}+a_{m+1}+\dots+a_{n} \\
\sum^{n+k}_{i=m+k}a_{i-k} & =a_{m}+a_{m+1}+\dots+a_{n} \\
\sum^{n-k}_{i=m-k}a_{i+k} & =a_{m}+a_{m+1}+\dots+a_{n}
\end{align}$$
# Properties of summation
## Facts
![[4.10 Sum Notation-1761666986239.jpeg]]
## Some proof sketches
i) $$\begin{align}
ca_{1}+c_{2}+\dots+ca_{n}=c (a_{1}+\dots+a_{n})
\end{align}$$
ii) $$\begin{align}
(a_{1}+b_{1})+\dots+(a_{n}+b_{n}) =(a_{1}+\dots+a_{n})+(b_{1}+\dots+b_{n})
\end{align}$$
iii) $$\begin{align}
\underbrace{ c+\dots+c }_{ \text{n times} }=n\cdot c
\end{align}$$
iv) $$\begin{align}
(\text{gauss age 10}) \\
s & =\sum ^n_{i=1}i=1+2+3+\dots+n-1+n \\
+s & =n+(n-1)+(n-2)+\dots+2+1 \\
 \\
2s & = \underbrace{ (n+1)+(n+1)+(n+1)+\dots+(n+1)+(n+1) }_{ \text{n terms} } \\
2s & =n(n+1) \\
s & =\frac{n(n+1)}{2}
\end{align}$$
# Examples
$$\begin{align}
\sum^{50}_{i=10}i & =\sum^{41}_{i=1}(i+9) \\
 & =\sum^{41}_{i=1}i+\sum^{41}_{i=1}9 \\
 & =\frac{41\cdot 42}{2}+41 \cdot 9 
\end{align}$$
$$\begin{align}
 & \lim_{ n \to \infty } \underbrace{ \sum^n_{i=1} \frac{3}{2} \left( \frac{i}{n}^3 +1\right) }_{ S } \\
s & =\sum^n_{i=1} \frac{3}{2} \left( \frac{i^3}{n^3}+1 \right) \\
 & =\frac{3}{n} \sum_{i+1}^n\left( \frac{i^3}{n^3} +1\right) \\
 & =\frac{3}{n} \left( \sum_{i+1}^n\frac{i^3}{n^3} +\underbrace{ \sum_{i+1}^n1 }_{ n }\right) \\
 & =\frac{3}{n} \left( \frac{1}{n^3} \sum_{i+1}^n i^3 +n\right)  \\
 & =\frac{3}{n}\left( \frac{1}{n^3}\left( \frac{n(n+1)}{2} \right)^2+n \right) \\
 & =\frac{3\cancel{ n^2 }(n+1)^2}{n^\cancel{ 4 }\cdot 4}+3 \\
 & \lim_{ n \to \infty } \frac{3(n+1)^2}{4n^2}+3 \\
 & \boxed{ =\frac{3}{4}+3 }
\end{align}$$
# Telescoping sums
$$\begin{align}
\sum_{i=1}^{50}\left( \frac{1}{i}-\frac{1}{i+1} \right) & =\left( \frac{1}{1}\cancel{ -\frac{1}{2} } \right)+\left( \cancel{ \frac{1}{2} }\cancel{ -\frac{1}{3} } \right)+\left( \cancel{ \frac{1}{3} }-\cancel{ \frac{1}{4} } \right)+\dots+\left( \cancel{ \frac{1}{50} }-\frac{1}{51} \right) \\
 & =1-\frac{1}{51}
\end{align}$$