# Example: Rational Function
$$\begin{align}
f(x)=\frac{2x^2}{x^2-1} 
\end{align}$$
## 1. Domain
$$\begin{align}
=(-\infty,-1)\cup(-1, 1)\cup(1,+\infty)
\end{align}$$
## 2. Intercepts
y-intercepts: $f(0)=0 \to (0,0)$
x-intercepts: $f(x)=0 \iff x=0$
## 3. Symmetry
$$\begin{align}
f(-x)=\frac{2(-x)^2}{(-x)^2-1}=\frac{2x^2}{x^2-1}=f(x) \\
\end{align}$$
our function is even
## 4. Asymptotes
### HA
$$\begin{align}
\lim_{ x \to \pm \infty } \frac{2x^2}{x^2-1}=2
\end{align}$$
### VA
$$\begin{align}
\lim_{ x \to 1^- } \frac{2x^2}{x^2-1}=\frac{2}{0^-} & =-\infty \\
\lim_{ x \to 1^+ } \frac{2x^2}{x^2-1}=\frac{2}{0^+} & =+\infty \\
\lim_{ x \to -1^- } \frac{2x^2}{x^2-1}=\frac{2}{0^-} & =+\infty \\
\lim_{ x \to -1^+ } \frac{2x^2}{x^2-1}=\frac{2}{0^+} & =-\infty
\end{align}$$
## 5. Increasing/Decreasing
$$\begin{align}
f'(x) & =\frac{d}{dx}\left( \frac{2x^2}{x^2-1} \right) \\
 & =\frac{4x(x^2-1)-2x^2\cdot 2x}{(x^2-1)^2} \\
 & =\frac{-4x}{(x^2-1)^2}
\end{align}$$
![[Untitled-1761061518909.jpeg]]
## 6. Concavity
$$\begin{align}
f''(x) & =\frac{d}{dx}\left( \frac{-4x}{(x^2-1)^2} \right) \\
 & =\frac{-4(x^2-1)^\cancel{ 2 }--4x\cdot 4x(\cancel{ x^2-1) }}{(x^2-1)^\cancel{ 4 }} \\
 & =\frac{-4x^2+4+16x^2}{(x^2-1)^3} \\
 & =\frac{12x^2+4}{(x^2-1)^3}
\end{align}$$
> [!NOTE] About derivatives
>  the derivative of a function will be the opposite (even -> odd), (odd -> even)

![[Untitled-1761061965220.jpeg]]
## 7. Conclusion
![[Untitled-1761061990117.jpeg]]
# Example: slant asymptote
## Definition:
A function f(x) has a slant asymptote y=mx+b if
$$\begin{align}
\lim_{ x \to \pm\infty }(f(x)-(mx+b))=0 
\end{align}$$
>[!NOTE] Fact:
>Rational functions have slant asymptotes if the degree of the numerator is one larger than the degree of the denominator
## Example
$$\begin{align}
  f(x) & =\frac{x^3-x^2+x+1}{x^2+1}=x-1+\frac{2}{x^2+1} \\
 & = \lim_{ x \to \pm\infty } (f(x)-(x-1)) \\
 & = \lim_{ x \to \pm\infty } \left( \frac{2}{x^2+1} \right) \\
 & = 0
\end{align}$$
![[4.5 - Summary of Curve Sketching-1761062573075.jpeg]]
# Example: Periodic Functions
## Question: What is the period of the following periodic function?
$$\begin{align}
 & f(x)=\sin x \implies 2\pi-\text{periodic} \\
 \\
 & g(x)=\frac{e^{\sin x}}{1+\cos^2(x)}=\frac{e^{\sin(x+2\pi)}}{1+\cos^2(x+2\pi)}=\frac{e^{\sin x}}{1+\cos^2x}=g(x)\implies 2\pi\text{ periodic} \\ \\

 & h(x)=\underbrace{ \sin(2x) }_{ \pi\text{ periodic} }+\underbrace{ \sin(4x) }_{ \frac{\pi}{2}\text{ periodic} }\implies \pi \text{ periodic}
\end{align}$$
## Complete the graph of sin(2x)+sin(4x)
![[4.5 - Summary of Curve Sketching-1761062993420.jpeg]]
## Bonus Question: discuss the symmetries of $f(x)=x+\sin x$
$$\begin{align}
f(-x)=-x+\sin(-x)=-x-\sin x=-f(x)\implies \text{odd}
\end{align}$$
