---
lastSync: Wed Feb 12 2025 02:52:27 GMT-0500 (Eastern Standard Time)
---
## First Equation
- $v_{f}=v_{i}+a\Delta t$
- this is the used to prove the other equations
- ==From the definition of acceleration==:
- Regular
	- $$a=\frac{\Delta v}{\Delta t}$$
	- $$a=\frac{vf-vi}{\Delta t}$$
	- $$a\Delta t=vf-vi$$
	- $$\boxed{vi=vf+a\Delta t}$$
- Calculus
	- $$a=\frac{dv}{dt}$$
	- $$\int_{ti}^{tf}adt=\int_{vi}^{vf}dv$$
	- $$at\Big|_{ti}^{tf}=v\Big|_{vi}^{vf}$$
	- $$at_{f}-at_{i}=v_{f}-v_{i}$$
	- $$a(t_{f}-t_{i})=v_{f}-v_{i}$$
	- $$a\Delta T=V_{f}-V_{i}$$
	- $$\boxed{V_{f}=V_{i}+a\Delta T}$$
## Second Equation
- From the V-T graph
- Standard Proof
	- $$\Delta d=A_{1}+A_{2}$$
	- $$\Delta d=V_{i}\Delta t+\frac{1}{2}(V_{f}-V_{i})(\Delta t)$$
	- But $V_{f}-V_{i}=a\Delta t$
	- $$\Delta d=V_{i}\Delta t+\frac{1}{2}(a\Delta t)(\Delta t)$$
	- $$\Delta d=V_{i}\Delta t+\frac{1}{2}(a\Delta t^2)$$
- Calculus Method
	- $$V=\frac{dx}{dt}$$
	- Sub in $V=V_{i}+at$ and integrate
	- $$V_{i}+at=\frac{dx}{dt}$$
	- $$\int(V_{i}+at)dt=\int dx$$
	- $$V_{i}t+\frac{at^2}{2}=x+C$$
	- at $t=0$ $x=x_{0}$
	- $\therefore c+x_{0}=0$
	- $c=-x_{0}$
	- $$V_{i}t+\frac{1}{2}at^2=x-x_{0}$$
	- $$\Delta x=V_{i}t+\frac{1}{2}at^2$$
## Third Equation
- Standard
	- $$\Delta d=A_{1}-A_{2}$$
	- $$\Delta d=(v_{f}\Delta t)-\frac{1}{2}(v_{f}-v_{i})(\Delta t)$$
	- $$\Delta d=(v_{f}\Delta t)-\frac{1}{2}(a\Delta t)(\Delta t)$$
	- $$\Delta d=v_{f}\Delta t-\frac{1}{2}a\Delta t^2$$
- Calculus
	- $$V=\frac{dx}{dt}$$
	- $$(v_{f}-at)=\frac{dx}{dt}$$
	- $$\int(v_{f}-at)dt=\int{dx}$$
	- $$v_{f}t-\frac{1}{2}at^2=x+c$$
	- at $t=0$ $x=x_{0}$
	- $\therefore c+x_{0}=0$
	- $c=-x_{0}$
	- $$v_{f}t-\frac{1}{2}at^2=\Delta x$$
## Fourth Equation
- Standard
	- $$A_{trapezium}=\frac{1}{2}(\text{sum of paralell sides})(\text{base})$$
	- $$\Delta d=\frac{1}{2}(v_{f}+v_{i})(\Delta t)$$
	- $$\Delta d=(\frac{v_{f}+v_{i}}{2})(\Delta t)$$
- Calculus
	- $$dx=Vdt$$
	- Need V in terms of 
	- $$y=mx+b$$
	- $$V=\left( \frac{v_{f}-v_{i}}{\Delta t} \right)t+v_{i}$$
	- $$V=\frac{dx}{dt}$$
	- $$\int_{x_{i}}^{x_{f}}\left(\left( \frac{v_{f}-v_{i}}{\Delta t} \right)t+v_{i}\right)dt=\int_{0}^t dx$$
	- $$x\Big|_{x_{i}}^{x_{f}}=\left( \frac{v_{f}-v_{i}}{\Delta t} \right)\frac{t^2}{2}+v_{i}t\Big|_{0}^t$$
	- $$\Delta x=\left( \frac{v_{f}-v_{i}}{t-0} \right)\frac{t^2}{2}+v_{i}t$$
	- $$\Delta x=\left( \frac{v_{f}-v_{i}}{2} \right)t+v_{i}t$$
	- $$\Delta x=\left( \frac{v_{f}-v_{i}}{2} \right)t+v_{i}t$$
## Fifth Equation
- Regular
	- $$vf=vi+a\Delta t$$
	- $$vf^2=(vi+a\Delta t)^2$$
	- $$vf^2=vi^2+2v_ia\Delta t+a^2t^2$$
	- $$vf^2=vi^2+2a\left( vit+\frac{1}{2} at^2\right)$$
	- $$vf^2=vi^2+2a\Delta d$$
- Calclulus
	- $$a=\frac{dv}{dt}$$
	- $$a=\frac{dv}{dx}\left( \frac{dx}{dt} \right)$$
	- $$a=\frac{dv}{dx}V$$
	- $$\int adx=\int vdv$$
	- $$ax=\frac{1}{2}v^2+c$$
	- at $x=x_{0}$, $v=v_{0}$
	- $$ax_{0}=\frac{1}{2}V_{0}+C$$
	- $$c=ax_{0}-\frac{1}{2}V_{0}^2$$
	- $$ax=\frac{1}{2}V^2+ax_{0}-\frac{1}{2}V^2$$
	- $$ax-ax_{0}=\frac{1}{2}V^2-\frac{1}{2}V_{0}^2$$