---
lastSync: Mon Mar 17 2025 13:19:31 GMT-0400 (Eastern Daylight Time)
---
## Lesson
- Expand and simplify
	- a)
		- $(a+b)^2=a^2+2ab+b^2$
	- b)
		- $(a+b)^3=(a^2+2ab+b^2)(a+b)$
		- $=(a^3+a^2b+2a^2b+2ab^2+ab^2+b^3)$
		- $=a^3+3a^2b+3ab^2+b^3$
	- c)
		- $(a+b)^4=(a+b)(a+b)(a+b)(a+b)$
		- $=(a^3+3a^2b+3ab^2+b^3)(a+b)$
		- $=a^4+a^3b+3a^3b+3a^2b^2+3a^2b^2+3ab^3+ab^3+b^4$
		- $=a^4+4a^3b+6a^2b^2+4ab^3+b^4$
	- d)
- What do you notice about your expansion and pascals triangle?
	- The coefficients of the expansion correlate with row $n$ of pascals triangle
- In general with $(a+b)^n$
	- What can you say about the number of terms in the expansion?
		- It is equal to n+1
		- The first term is $a^n$ and the last term is $b^n$
	- What is true about the sum of exponents in each term of the expansion?
		- The exponents sums of each term in $n$
	- What is the relation between the term number of the expansion and the exponent of b?
		- The exponent of b is one less than the term number
- Using your pascals triangle, expand and simplify the following
	- $(a+b)^6$
		- $= 1+6+15+20+15+6+1$
		- $=1a^6+6a^5+15a^4+20a^3+15a^2+6a+1$
		- $=1a^6+6a^5b+15a^4b^2+20a^3b^3+15a^2b^4+6ab^5+1b^6$
	- $(3x-2y)^5$
		- $=1+5+10+10+5+1$
		- $=1(3x)^5+5(3x)^4+10(3x)^3+10(3x)^2+5(3x)^1+1$
		- $=1(3x)^5+5(3x)^4(-2y)+10(3x)^3(-2y)^2+10(3x)^2(-2y^3)+5(3x)^1(-2y)^4+1(-2y)^5$
		- $=243x^5-810x^4y+1080x^3y^2-720x^2y^3+240xy^4-32y$