# Problem Set
- 1) - D
$$\begin{align}
\frac{1}{1-\cos \theta}+\frac{1}{1+\cos \theta} & = \frac{1-\cos \theta+1+\cos \theta}{(1-\cos \theta)(1+\cos \theta)} \\
 & = \frac{2}{1-\cos ^2 \theta} \\
 & =\frac{2}{\sin^2 \theta} \\
 & \boxed{ =2 \csc^2 \theta }
\end{align}$$
- 2) - E
$$\begin{align}
\boxed{ \lim_{ x \to -4^- } \neq \lim_{ x \to -4^+ } \therefore D.N.E  }
\end{align}$$
- 3) - C
- 4) - C
$$\begin{align}
 & \lim_{ x \to 4 } \frac{f(x)^2}{f(x)-g(x)}=12 \\
\iff  & \frac{f(4)^2}{f(4)-3}=12 \\
\iff & f(4)^2=12f(4)-12(3) \\
\iff & f(4)^2-12f(4)+12(3)=0 \\
\iff & \boxed{ f(4)=6 }
\end{align}$$
- 5) - A
$$\begin{align}
 & \csc \theta =\frac{5}{1}  \\
 \implies  & \sin \theta=\frac{1}{5} \\
 \implies  & \cos \theta=\frac{\sqrt{ 24 }}{5} \\ \\

\implies  & \sin 2\theta=2\cos \theta \sin \theta \\
\iff & 2\left( \frac{1}{5} \right)\left( \frac{\sqrt{ 24 }}{5} \right) \\
\iff & \boxed{ \frac{2\sqrt{ 24 }}{25} }
\end{align}$$
- 6) - A
$$\begin{align}
\arctan \frac{1}{\sqrt{ 3 }} & = \frac{\pi}{3}, \frac{4\pi}{3}
\end{align}$$
- 7) - E
$$\begin{align}
\text{every answer would give a transcendental number answer}
\end{align}$$
- 8) - D
$$\begin{align}
 1-x & \geq0 \\
 1 & \geq x \\
 \\
5-\sqrt{ 1-x } & >0 \\
5 & >\sqrt{ 1-x } \\
25 & >1-x \\
x & >-24 \\
 \\
 & \boxed{ \{ x|-24<x\leq 1 \} }
\end{align}$$
- 9) - C
$$\begin{align}
\boxed{ \sec \frac{5\pi}{3}=2 }
\end{align}$$
- 10) - A
$$\begin{align}
\cos(\arcsin x) & \impliedby \cos \theta=\sqrt{ 1-\sin^2\theta }, \theta=\arcsin x \\
 & \implies\boxed{  \cos x=\sqrt{ 1-x^2 } }
\end{align}$$
- 11) - A
$$\begin{align}
\lim_{ x \to 0 } \frac{2-\sqrt{ 4-x^2 }}{3x}  & = \frac{\frac{1}{-2\sqrt{ 4-x^2 }}(-2x)}{3} \\
 & \boxed{ =0 }\\
\end{align}$$
- 12) - D
$$\begin{align}
\ln(5^x-1) & =3 \\
5^x-1 & =e^3 \\
5^x & =e^3-1 \\
x\ln 5 & =\ln (e^3-1) \\
x & = \boxed{ \frac{\ln(e^3-1)}{\ln 5} }
\end{align}$$
- 13) - B
$$\begin{align}
2\cos^2\theta & =1 \\
\cos \theta & =\pm \sqrt{ \frac{1}{2} } \\
\theta & =\boxed{ \frac{\pi}{4}, \frac{3\pi}{4}, \frac{5\pi}{4}, \frac{7\pi}{4} }
\end{align}$$
- 14) - E
$$\begin{align}
f(x) & =e^{-(x+3)} \\
 x & =e^{-(y+3)} \\
\ln x & =-y-3 \\
y & =-3-\ln x
\end{align}$$
- 15) - E
$$\begin{align}
\lim_{ h \to 0 } \frac{\ln(1+h)}{h} & =\lim_{ h \to 0 } \frac{\ln (1+h)+\ln 1}{h}
\end{align}$$
- 16) - D
$$\begin{align}
\left( \frac{g}{f^2+g} \right)' & =\frac{g'(f^2+g)-g(2f\times f'+g')}{(f^2+g)^2} \\
 & =\frac{(-3)((-1)^2+(5))-(5)(2(-1)\times (2)+(-3))}{((-1)^2+5)^2} \\
 & = \frac{17}{36}
\end{align}$$
- 17) - A
$$\begin{align}
\frac{d}{dx}(x^2h(x)) & =x^2h'(x)+2xh(x) \\
 & =4^2(7)+2(4)(-3) \\
 & =88
\end{align}$$
- 18) - E
$$\begin{align}
v'(1) & =g'(f(x)) \times f'(x) \\
 & =
\end{align}$$
- 19) - 
$$\begin{align}
\lim_{ x \to \infty } \arctan\left( \frac{4x^2+3x}{6x^3+x} \right) & =\arctan(\lim_{ x \to \infty }\frac{4x^2+3x}{6x^3+x} ) \\
 & = \arctan(0) \\
 & = 0
\end{align}$$
- 20) - E
- 21) - D
$$\begin{align}
y' & =\sec x\tan x+2\sin x \\
f\left( \frac{\pi}{3} \right) & = \sec \frac{\pi}{3}\tan \frac{\pi}{3}+2\sin \frac{\pi}{3}=3 \, \sqrt{3}
\end{align}$$
- 22) - B
- 23) - D
$$\begin{align}
r^2e^{rx}+6re^{rx}-7e^{rx} & =0 \\
 e^{rx}(r^2+6r-7) & =0 \\
\boxed{ r=1, -7 }

\end{align}$$
- 24) - D
$$\begin{align}
f(x) & =2\sin x+\sin^2x \\
f'(x) & =2\cos x+\sin 2x \\
 0 & =2\cos x+\sin 2x \\
 0 & =2\cos x(1+\sin x) \\
 \\
0 & =\cos x \\
1 & =\sin x \\
 \\
x & =\frac{\pi}{2}, \frac{3\pi}{2}
\end{align}$$
- 72) - D
$$\begin{align}
 & e^{x-y^2}(1-2y\times y')=\frac{y'(1+e^{x^2})-y(2e^{x^2}x)}{(1+e^{x^2})^2} \\
\iff  & e^{x-y^2}-2y\times y'\times e^{x-y^2}=\frac{y'(1+e^{x^2})}{(1+e^{x^2})^2}-\frac{y(2e^{x^2}x)}{(1+e^{x^2})^2} \\
\iff  & e^{x-y^2}-\frac{y(2e^{x^2}x)}{(1+e^{x^2})^2}=\frac{y'(1+e^{x^2})}{(1+e^{x^2})^2}+2y\times y'\times e^{x-y^2} \\
\iff & e^{x-y^2}-\frac{y(2e^{x^2}x)}{(1+e^{x^2})^2}=y'\left( \frac{(1+e^{x^2})}{(1+e^{x^2})^2}+2y e^{x-y^2} \right) \\
\iff  & \frac{e^{x-y^2}-\frac{y(2e^{x^2}x)}{(1+e^{x^2})^2}}{\left( \frac{1}{(1+e^{x^2})}+2y e^{x-y^2} \right)}=y'

\end{align}$$