- 1) - D
$$\begin{align}
x & =\frac{1}{3}\ln(2-\ln y) \\
3x & =\ln(2-\ln y) \\
e^{3x} & =2-\ln y \\
y & =e^{2-e^{3x}}
\end{align}$$
- 2) - C
$$\begin{align}
\sec x\csc x & = \frac{1}{\cos x} \frac{1}{\sin x} \\
 & =\frac{1}{\cos x\sin x} \\
 & =\frac{2}{2\cos x\sin x} \\
 & =\frac{2}{\sin 2x} \\
 & =2\csc 2x
\end{align}$$
- 3) - A
- 4) - B
$$\begin{align}
f'(x) & =\frac{1}{\sec x} \times \sec x\tan x-2\sin x \\
 & = \tan x-2\sin x \\
 & =\frac{\sin x}{\cos x}-2\sin x \\
 & =\frac{\sin x-2\sin x\cos x}{\cos x} \\
 & =\frac{\sin x(1-2\cos x)}{\cos x} \\
 \\
 & \sin x=0 \\
 & x=0, \pi, 2\pi \\
 \\
 & \cos x=\frac{1}{2} \\
 & x=\frac{\pi}{3}, \frac{5\pi}{3}
\end{align}$$
- 5) - B
$$\begin{align}
g(-6) & =8 \\
8 & =3x+5^x \\
8 & =3(1)+5^1
\end{align}$$
- 6) - A
- 7) - C
$$\begin{align}
\lim_{ x \to a }  & \frac{f(x)-f(a)}{x-a} \\
\lim_{ x \to 2 } &  \frac{x^4-x-3-f(2)}{x-2} \\
\lim_{ x \to 2 }  & \frac{x^4-x-14}{x-2} \\
 \\
\lim_{ h \to 0 }  & \frac{(x+h)^4-(x+h)-3-x^4+x+3}{h} \\
\lim_{ h \to 0 }  & \frac{(2+h)^4-h-16}{h}
\end{align}$$
- 8) - B
$$\begin{align}
h'(4) & =(4+\sqrt{ 4^3 })\left( \frac{1}{3} \right)+\left( \frac{3}{2}4^{1/2} \right)(1) \\
 & =7
\end{align}$$
- 9) - C
$$\begin{align}
\lim_{ x \to 2 } \frac{x^2-4}{\sqrt{ x +2 }-2}=16
\end{align}$$
- 10) - D
- 11) - C
$$\begin{align}
f'(4) & =\frac{x'g(4)-xg'(4)}{g(4)^2} \\
 & = \frac{2-4(-3)}{4} \\
 & = \frac{14}{4} \\ \\
 y & =\frac{14}{4}x+b \\
2 & =\frac{14}{4}4+b \\
b & =-12
\end{align}$$
- 12) - E
- 13) - C
$$\begin{align}
y & =(1+x^2)^x \\
\ln y & =x\ln(1+x^2) \\
\frac{y'}{y} & =\frac{d}{dx}x\ln (1+x^2) \\
\frac{y'}{y}& = \ln(1+x^2)+x \frac{1}{1+x^2}(2x) \\
y' & =y(\ln(1+x^2)+x \frac{1}{1+x^2}(2x)) \\
f'(1) & =2(\ln 2+1)
\end{align}$$
- 14) - D
$$\begin{align}
y & =e^{\tan^2x} \\
\frac{y'}{y} & = \frac{d}{dx}\tan^2x \\
y' & =y \times 2 \frac{\sin x}{\cos x}  \times \frac{1}{\cos^2x}   \\
y' & =e^{\tan^2x}\left( \frac{2\sin x}{\cos^3x} \right) \\
f'\left( \frac{\pi}{4} \right) & =e\left( \frac{\frac{2}{\sqrt{ 2 }}}{\frac{1}{\sqrt{ 2 }^3}} \right) \\
f'\left( \frac{\pi}{4} \right) & =e\left( \frac{2}{\frac{1}{2}} \right) \\
 & =4e
\end{align}$$
$$\begin{align}
\end{align}$$
- **15) - B**
$$\begin{align}
xy'+y & =-20+3y^2y' \\
y+20 & = 3y^2y'-xy' \\
\frac{y+20}{3y^2-x} & =y' \\
 \\
64 & =y^3 \\
4 & =y \\
 \\
\frac{4+20}{3(4)^2} & =\frac{24}{48}=\frac{1}{2}
\end{align}$$
- 16) - B
- 17) - E
$$\begin{align}
6 \left( \frac{e^x-e^{-x}}{2} \right)+8\left( \frac{e^x+e^{-x}}{2} \right) & =3e^x-3e^{-x}+4e^x+4e^{-x} \\
 & =7e^x+e^{-x}
\end{align}$$
- 18) - A
$$\begin{align}
x_{2} & =2-\frac{f(2)}{f'(2)} \\
 \\
f(2) & = 9 \\
 \\
f'(2) & = h'(g(x))g'(x) \\
 & =3(-1) \\
 \\
x_{2} & =2-\frac{9}{-3} \\
x_{2} & =5
\end{align}$$
- 19) - A
$$\begin{align}
f(x) & =x^3(1-x)^9 \\
 & =3x^2(1-x)^9+x^3(-9(1-x)^8) \\
 & =x^2(3(1-x)^9+x(-9(1-x)^8)) \\
 & =x^2((1-x)^8(3(1-x)-9x)) \\
 & =x^2(1-x^8)(3(1-4x)) \\
x & =0, 1, \frac{1}{4}
\end{align}$$
- 20) - D
$$\begin{align}
f(-1)'(7) \\
 \\
f-1(7)=3 \\
f(3)=7 \\
x=3 \\
f'(3)=\frac{1}{2}
\end{align}$$